Soundness.thy
@@ -111,6 +111,18 @@ lemma act_not_eq_iff[simp]:
 
 subsection \<open> Operational semantics steps \<close>
 
+fun head_atoms :: \<open>'a comm \<Rightarrow> ('a \<Rightarrow> 'a \<Rightarrow> bool) set\<close> where
+  \<open>head_atoms (c1 ;; c2) = (let a1 = head_atoms c1
+                             in if a1 = \<bottom> then head_atoms c2 else a1)\<close>
+| \<open>head_atoms (c1 \<^bold>+ c2) = (head_atoms c1 \<squnion> head_atoms c2)\<close>
+| \<open>head_atoms (c1 \<box> c2) = (head_atoms c1 \<squnion> head_atoms c2)\<close>
+| \<open>head_atoms (c1 \<parallel> c2) = (head_atoms c1 \<squnion> head_atoms c2)\<close>
+| \<open>head_atoms (Atomic b) = {b}\<close>
+| \<open>head_atoms (c\<^sup>\<star>) = head_atoms c\<close>
+| \<open>head_atoms Skip = {}\<close>
+| \<open>head_atoms (\<mu> c) = head_atoms c\<close>
+| \<open>head_atoms (FixVar x) = \<bottom>\<close>
+
 inductive opstep :: \<open>act \<Rightarrow> ('l \<times> 's) \<times> ('l \<times> 's) comm \<Rightarrow> (('l \<times> 's) \<times> ('l \<times> 's) comm) \<Rightarrow> bool\<close> where
   seq_left[intro!]: \<open>opstep a (h, c1) (h', c1') \<Longrightarrow> opstep a (h, c1 ;; c2) (h', c1' ;; c2)\<close>
 | seq_right[intro!]: \<open>opstep Tau (h, Skip ;; c2) (h, c2)\<close>
@@ -120,11 +132,13 @@ inductive opstep :: \<open>act \<Rightarrow> ('l \<times> 's) \<times> ('l \<tim
 | endet_tau_right[intro]: \<open>opstep Tau (h, c2) (h', c2') \<Longrightarrow> opstep Tau (h, c1 \<box> c2) (h', c1 \<box> c2')\<close>
 | endet_skip_left[intro!]:  \<open>opstep Tau (h, Skip \<box> c2) (h, c2)\<close>
 | endet_skip_right[intro!]: \<open>opstep Tau (h, c1 \<box> Skip) (h, c1)\<close>
-| endet_local_left[intro]:  \<open>opstep Local (h, c1) s' \<Longrightarrow> opstep Local (h, c1 \<box> c2) s'\<close>
-| endet_local_right[intro]: \<open>opstep Local (h, c2) s' \<Longrightarrow> opstep Local (h, c1 \<box> c2) s'\<close>
+| endet_local_left[intro]:  \<open>a \<noteq> Tau \<Longrightarrow> opstep a (h, c1) s' \<Longrightarrow> opstep a (h, c1 \<box> c2) s'\<close>
+| endet_local_right[intro]: \<open>a \<noteq> Tau \<Longrightarrow> opstep a (h, c2) s' \<Longrightarrow> opstep a (h, c1 \<box> c2) s'\<close>
 | par_left[intro]: \<open>opstep a (h, s) (h', s') \<Longrightarrow> opstep a (h, s \<parallel> t) (h', s' \<parallel> t)\<close>
 | par_right[intro]: \<open>opstep a (h, t) (h', t') \<Longrightarrow> opstep a (h, s \<parallel> t) (h', s \<parallel> t')\<close>
 | par_skip[intro!]: \<open>opstep Tau (h, Skip \<parallel> Skip) (h, Skip)\<close>
+| iter_step[intro]: \<open>opstep a (h, c) (h', c') \<Longrightarrow> opstep a (h, c\<^sup>\<star>) (h, c' ;; c\<^sup>\<star>)\<close>
+| iter_end[intro]: \<open>\<not> pre_state (\<Squnion>(head_atoms c)) h \<Longrightarrow> opstep a (h, c\<^sup>\<star>) (h, Skip)\<close>
 | fixpt_skip[intro!]: \<open>c' = c[0 \<leftarrow> \<mu> c] \<Longrightarrow> opstep Tau (h, \<mu> c) (h, c')\<close>
 | atomic[intro!]: \<open>a = Local \<Longrightarrow> snd s' = Skip \<Longrightarrow> b h (fst s') \<Longrightarrow> opstep a (h, Atomic b) s'\<close>
 
